refractoring, more instances.
1) added the L5 to L6 translation instance in L6_PCPS/classes.v
2) L6_PCPS is now in the namespace L6 instead of "". Otherwise it seemed impossible to avoid filename clashes (almost every directory now has classes.v).
It would be good to fully qualify the imports of L6 files as L6.xxx

theories/common/certiClasses.v
@@ -48,6 +48,15 @@ Definition bigStepPreserving `{CerticoqTranslation Src Dst}
     -> s ⇓ sv
     -> (translate Src Dst s) ⇓ (translate Src Dst sv).
 
+Arguments bigStepPreserving Src Dst {H} {H0} {H1} {H2}.
+
+(* Sometimes, the translation of a value may not be a value. 
+For example, in L3 to L4, the environment is translated as let bindings.
+Thus, a value with a non-empty environment will be translated to a term
+whose outermost operator is a let binding and is hence not a value.
+This definition, which is inspired by CPS correct seems weaker, is not strong enough
+to be sensible. For example it is possible that the translation of [s] and [sv] both
+diverge. *)
 Definition bigStepPreservingWeaker `{CerticoqTranslation Src Dst}
    `{BigStepOpSem Src} `{BigStepOpSem Dst} `{WellFormed Src}
   :=
@@ -56,8 +65,8 @@ Definition bigStepPreservingWeaker `{CerticoqTranslation Src Dst}
     -> s ⇓ sv
     -> ((translate Src Dst s) ⇓ (Ret tv) <-> (translate Src Dst sv) ⇓ (Ret tv)).
 
+Arguments bigStepPreservingWeaker Src Dst {H} {H0} {H1} {H2}.
 
-Arguments bigStepPreserving Src Dst {H} {H0} {H1} {H2}.
 
 (** A Certicoq language must have an associated bigstep operational semantics and 
   a well formedness predicate (possibly \_.True) *)
@@ -109,11 +118,6 @@ Proof.
   assumption.
 Qed.
 
-Instance  BigStepOpWEnv (Term:Set) (ev: (environ Term) -> Term -> Term -> Prop) :
-  BigStepOpSem (Program Term) :=
-fun p1 p2 => ev (env p1) (main p1) (main p2) /\ (env p1 = env p2).
-
-
 
 Instance composeCerticoqTranslationCorrect (Src Inter Dst: Type)
   `{CerticoqLanguage Src}
@@ -136,6 +140,40 @@ Proof.
   exact Hev.
 Qed.
 
+
+Instance  BigStepOpWEnv (Term:Set) (ev: (environ Term) -> Term -> Term -> Prop) :
+  BigStepOpSem (Program Term) :=
+fun p1 p2 => ev (env p1) (main p1) (main p2) /\ (env p1 = env p2).
+
+
+(* A possible replacement for [CerticoqTranslationCorrect] 
+Class CerticoqTranslationCorrect2 
+  `{CerticoqLanguage Src} `{CerticoqLanguage Dst}
+  `{CerticoqTranslation Src Dst} := 
+{
+  certiWfPres2 : wfPreserving Src Dst;
+  certiBigStepPres2 : bigStepPreservingWeaker Src Dst;
+}.
+
+Arguments CerticoqTranslationCorrect2 Src {H} {H0} {H1} Dst {H2} {H3} {H4} {H5}.
+
+
+Instance composeCerticoqTranslationCorrect2 (Src Inter Dst: Type)
+  `{CerticoqLanguage Src}
+  `{CerticoqLanguage Inter}
+  `{CerticoqLanguage Dst}
+  {t1 : CerticoqTranslation Src Inter}
+  {t2 : CerticoqTranslation Inter Dst}
+  {Ht1: CerticoqTranslationCorrect2 Src Inter}
+  {Ht2: CerticoqTranslationCorrect2 Inter Dst}
+    : CerticoqTranslationCorrect2 Src Dst.
+Proof.
+  destruct Ht1, Ht2.
+  constructor;[eapply composePreservesWf; eauto|].
+  intros ? ? ? Hwf Hev.
+  specialize (fun ti => certiBigStepPres3 _ _ ti Hwf Hev).
+
+*)
 
 
 (* ( * ) in Randy's email dated Tue, May 31, 2016 at 10:35 PM EST 
