theories/L6_PCPS/classes.v
@@ -1,0 +1,36 @@
+Require Export CPS.cpseval.
+
+Require Import cps.
+Require Import cps_util.
+
+
+Require Import certiClasses.
+Require Import Common.Common.
+
+(* Fix. L6 bigstep eval (L6.eval.bigstep_e) is strange it is a hetergenous relation of type
+  [env -> cps.exp -> val -> nat].
+  Perhaps the L6 term type should be (env * (cps.exp + cps.val)) 
+  bigstep_e counts costs, which is not a problem because we can existentially quantify 
+  over the count.
+*)
+Instance bigStepOpSemL3Term : BigStepOpSem cps.exp :=
+  fun _ _ => True.
+
+(* Fix *)
+Instance WfL3Term : WellFormed cps.exp :=
+  fun p  => True .
+
+Instance certiL6 : CerticoqLanguage cps.exp := {}.
+
+Require Import L4.classes.
+Require Import L5_to_L6.
+
+Instance certiL5a_t0_L6: 
+  CerticoqTranslation L5a.cps cps.exp :=
+fun x => Ret (convert_top x).
+
+
+
+
+
+
